msl_ext/log_normalize.v
@@ -7,6 +7,66 @@ Require Import VST.msl.log_normalize.
 
 Local Open Scope logic.
 
+Lemma allp_uncurry: forall {A} `{NatDed A} (S T: Type) (P: S -> T -> A),
+  allp (fun s => allp (P s)) = allp (fun st => P (fst st) (snd st)).
+Proof.
+  intros.
+  apply pred_ext.
+  + apply allp_right; intros [s t].
+    apply (allp_left _ s).
+    apply (allp_left _ t).
+    apply derives_refl.
+  + apply allp_right; intro s.
+    apply allp_right; intro t.
+    apply (allp_left _ (s, t)).
+    apply derives_refl.
+Qed.
+
+Lemma allp_curry: forall {A} `{NatDed A} (S T: Type) (P: S * T -> A),
+  allp P = allp (fun s => allp (fun t => P (s, t))).
+Proof.
+  intros.
+  apply pred_ext.
+  + apply allp_right; intro s.
+    apply allp_right; intro t.
+    apply (allp_left _ (s, t)).
+    apply derives_refl.
+  + apply allp_right; intros [s t].
+    apply (allp_left _ s).
+    apply (allp_left _ t).
+    apply derives_refl.
+Qed.
+
+Lemma exp_uncurry: forall {A} `{NatDed A} (S T: Type) (P: S -> T -> A),
+  exp (fun s => exp (P s)) = exp (fun st => P (fst st) (snd st)).
+Proof.
+  intros.
+  apply pred_ext.
+  + apply exp_left; intro s.
+    apply exp_left; intro t.
+    apply (exp_right (s, t)).
+    apply derives_refl.
+  + apply exp_left; intros [s t].
+    apply (exp_right s).
+    apply (exp_right t).
+    apply derives_refl.
+Qed.
+
+Lemma exp_curry: forall {A} `{NatDed A} (S T: Type) (P: S * T -> A),
+  exp P = exp (fun s => exp (fun t => P (s, t))).
+Proof.
+  intros.
+  apply pred_ext.
+  + apply exp_left; intros [s t].
+    apply (exp_right s).
+    apply (exp_right t).
+    apply derives_refl.
+  + apply exp_left; intro s.
+    apply exp_left; intro t.
+    apply (exp_right (s, t)).
+    apply derives_refl.
+Qed.
+
 Lemma sepcon_left1_corable_right: forall {A} `{CorableSepLog A} P Q R, corable R -> P |-- R -> P * Q |-- R.
 Proof.
   intros.
@@ -64,6 +124,15 @@ Proof.
   apply sepcon_derives; apply (exp_right x); apply derives_refl.
 Qed.
 
+Lemma precise_left_sepcon_andp_sepcon: forall {A} `{PreciseSepLog A} P Q R, precise P -> (P * Q) && (P * R) |-- P * (Q && R).
+Proof.
+  intros.
+  eapply derives_trans.
+  + apply precise_left_sepcon_andp_distr with P; auto.
+  + apply sepcon_derives; auto.
+    apply andp_left1; auto.
+Qed.
+
 Lemma precise_exp_sepcon: forall {A} `{PreciseSepLog A} {B} (P Q: B -> A), precise (exp P) -> precise (exp Q) -> precise (exp (P * Q)).
 Proof.
   intros.
@@ -101,12 +170,71 @@ Proof.
   apply TT_right.
 Qed.
 
+Lemma emp_disj: forall {A} {ND: NatDed A} {SL: SepLog A} {PSL: PreciseSepLog A} {OSL: OverlapSepLog A} {DSL: DisjointedSepLog A} P, disjointed emp P.
+Proof.
+  intros.
+  apply disj_comm, disj_emp.
+Qed.
+
+Lemma disj_FF: forall {A} {ND: NatDed A} {SL: SepLog A} {PSL: PreciseSepLog A} {OSL: OverlapSepLog A} {DSL: DisjointedSepLog A} P, disjointed P FF.
+Proof.
+  intros.
+  eapply disj_derives; [| | apply disj_emp].
+  apply derives_refl.
+  apply FF_left.
+Qed.
+
+Lemma FF_disj: forall {A} {ND: NatDed A} {SL: SepLog A} {PSL: PreciseSepLog A} {OSL: OverlapSepLog A} {DSL: DisjointedSepLog A} P, disjointed FF P.
+Proof.
+  intros.
+  apply disj_comm, disj_FF.
+Qed.
+
+Lemma disj_ocon_left: forall {A} {ND: NatDed A} {SL: SepLog A} {PSL: PreciseSepLog A} {OSL: OverlapSepLog A} {DSL: DisjointedSepLog A} P Q R, disjointed Q P -> disjointed R P -> disjointed (ocon Q R) P.
+Proof.
+  intros.
+  apply disj_comm.
+  apply disj_comm in H.
+  apply disj_comm in H0.
+  apply disj_ocon_right; auto.
+Qed.
+
 Lemma disj_sepcon_right: forall {A} {ND: NatDed A} {SL: SepLog A} {PSL: PreciseSepLog A} {OSL: OverlapSepLog A} {DSL: DisjointedSepLog A} P Q R, disjointed P Q -> disjointed P R -> disjointed P (Q * R).
 Proof.
   intros.
   pose proof disj_ocon_right _ _ _ H H0.
   eapply disj_derives; [apply derives_refl | | exact H1].
   apply sepcon_ocon.
+Qed.
+
+Lemma disj_sepcon_left: forall {A} {ND: NatDed A} {SL: SepLog A} {PSL: PreciseSepLog A} {OSL: OverlapSepLog A} {DSL: DisjointedSepLog A} P Q R, disjointed Q P -> disjointed R P -> disjointed (Q * R) P.
+Proof.
+  intros.
+  apply disj_comm.
+  apply disj_comm in H.
+  apply disj_comm in H0.
+  apply disj_sepcon_right; auto.
+Qed.
+
+Lemma disj_prop_andp_left: forall {A} {ND: NatDed A} {SL: SepLog A} {PSL: PreciseSepLog A} {OSL: OverlapSepLog A} {DSL: DisjointedSepLog A} (P: Prop) Q R, ({P} + {~ P}) -> (P -> disjointed Q R) -> disjointed ((!! P) && Q) R.
+Proof.
+  intros.
+  destruct H.
+  + apply H0 in p.
+    eapply disj_derives; [ | | exact p].
+    - apply andp_left2, derives_refl.
+    - apply derives_refl.
+  + eapply disj_derives; [ | | apply FF_disj].
+    - apply andp_left1. normalize.
+    - apply derives_refl.
+Qed.
+
+Lemma disj_prop_andp_right: forall {A} {ND: NatDed A} {SL: SepLog A} {PSL: PreciseSepLog A} {OSL: OverlapSepLog A} {DSL: DisjointedSepLog A} (P: Prop) Q R, ({P} + {~ P}) -> (P -> disjointed R Q) -> disjointed R ((!! P) && Q).
+Proof.
+  intros.
+  apply disj_comm.
+  apply disj_prop_andp_left; auto.
+  intros; apply disj_comm; auto.
 Qed.
 
 Lemma mapsto_precise: forall {AV: AbsAddr} {A} {mapsto: Addr -> Val -> A} {ND: NatDed A} {SL: SepLog A} {PSL: PreciseSepLog A} {MSL: MapstoSepLog AV mapsto} p v , precise (mapsto p v).
